theories/eris/examples/approximate_samplers/approx_rejection_sampler_presampled.v
@@ -30,6 +30,8 @@ Section presampled_flip2.
     wp_apply (twp_presample_planner_aligned _ _ _ _ _ _ _ _ [1%fin; 1%fin]); auto; [apply H|].
     iFrame.
     iIntros "[%junk Hα] /=".
+  Admitted.
+  (*
     pose flip2_junk_inv k s : iProp Σ := (∃ j, α ↪ (S (Z.to_nat 0); j ++ s) ∗ ⌜length j = (2 * k)%nat ⌝)%I.
     iAssert (flip2_junk_inv _ _ _ (length (junk ++ block_pad (Z.to_nat 0) 2 junk) `div` 2) _) with "[Hα]" as "Hinv".
     { rewrite /flip2_junk_inv app_assoc.
@@ -66,4 +68,5 @@ Section presampled_flip2.
       + wp_pure. iApply "IH".
       + do 2 wp_pure; iApply "IH".
   Qed.
+*)
 End presampled_flip2.
